subcomp added to effect

Probabilism.fst
@@ -1,15 +1,18 @@
 module Probabilism
 
 open FStar.Real
-
-let pr = p:real{p >=. 0.0R}
+open FStar.List.Tot
+  
+unfold let pr = p:real{p >=. zero}
 let prob_post (a:Type) = a -> Tot pr
-let prob_pre = pr
+unfold let prob_pre = pr
 let prob_wp (a:Type) = prob_post a -> Tot prob_pre
 
 assume type distribution (a:Type) : Type
 
 assume val point_distribution (#a:Type) (x:a) : distribution a
+
+assume val uniform_distribution (#a:Type) (x:list a{Cons? x}) : distribution a
 
 let prob (a:Type) (w:prob_wp a): Tot Type0 =
   distribution a // TODO: require w to hold
@@ -25,11 +28,31 @@ let prob_bind a b (w1:prob_wp a) (w2:a -> prob_wp b)
       (f: prob a w1) (g: (x:a -> prob b (w2 x))) : prob b (prob_wbind a b w1 w2) =
    admit()   
 
+let cast a (x:a) = x
+
+// let blabla #a (w1 w2 : prob_wp a) : Type0 = (forall (p:prob_post a). (w2 p <=. w1 p))
+
+let prob_stronger #a (w1 w2:prob_wp a) = forall x. w1 x <=. w2 x
+
+let prob_subcomp a (#w1 #w2 : prob_wp a) (f:prob a w1) : 
+                 Pure (prob a w2) (requires w2 `prob_stronger` w1) (ensures (fun _ -> True)) =
+  f
+
+//let stronger_refl #a (w:prob_wp a): Lemma(w `prob_stronger` w) = ()
+
+let ite_prob a (#w1 #w2 : prob_wp a) (f: prob a w1) (g: prob a w2) (b: bool) : Type =
+  prob a (if b then w1 else w2)
+
+// [@@allow_informative_binders] // Can we get rid of this and still have reifiable?
+total
+//reifiable
 reflectable
 layered_effect { PROB : (a:Type) -> (wp:prob_wp a) -> Effect with 
   repr = prob;
   return = prob_return; 
-  bind = prob_bind
+  bind = prob_bind;
+  subcomp = prob_subcomp;
+  if_then_else = ite_prob
   }
 
 unfold
@@ -45,17 +68,58 @@ let lift_pure_prob (a:Type) (#pwp:prob_wp a) (wp:pure_wp a) (f: eqtype_as_type u
    
 sub_effect PURE ~> PROB = lift_pure_prob
 
-unfold
-let goal = (Probabilism.compatible (fun p ->
-             forall (return_val: Prims.string). return_val == "hello" ==> p return_val)
-         (fun p -> p "hello"))
-
 let hint a : squash(forall (y x:a). (forall post. post y ==> post x) ==> (x == y)) = admit()
 
 let hint_string () = hint string
 
+let average (l:list pr{Cons? l}) : pr =
+  assume False;
+  (fold_left (fun pr x -> pr +. x) zero l) /. of_int (length l)
+
+let pick #a (l:list a{Cons? l}) : PROB a (fun post -> average (map post l)) =
+  PROB?.reflect (uniform_distribution l)
+
+let coin () : PROB bool (fun post -> (post true +. post false) /. two) =
+  PROB?.reflect (uniform_distribution [true;false])
+
+(**** TESTS *****)
+
+let test1 () : PROB bool (fun p -> (p true +. p false) /. two) = coin ()
+
+let test2 () : PROB bool (fun p -> zero) = coin ()
+
 let test3 x : PROB string (fun p -> p x) = x
 
-let test2 () : PROB string (fun post -> post "hello") = test3 "hello"
+let test4 () : PROB string (fun post -> post "hello") = test3 "hello"
+
+let f (b:bool) : nat = if b then 0 else 1
+
+let return (#a) (x:a) : PROB a (fun p -> p x) = 
+  PROB?.reflect (prob_return a x)
+
+let test5 () : PROB nat (fun p -> (p 0 +. p 1) /. two) =
+  let c : bool = coin() in
+  return (f c)
+
+// FAILS
+(* let test6 () : PROB nat (fun p -> (p 0 +. p 1) /. two) =
+  let c : bool = coin() in
+  return (if c then 0 else 1) *)
+
+// FAILS
+(* let test7 () : PROB nat (fun p -> (p 0 +. p 1) /. two) =
+  let c : bool = coin() in
+  f c *)
+
+let prob_unit : prob_wp unit = fun p -> p ()
+
+// FAILS
+(* let test7 () : PROB nat (fun p -> (p 0 +. p 1) /. two) =
+  let c : bool = coin() in
+  (if c then return 0 else return 1) *)
+
 
 // let reified = reify (test2 ())
+
+// let coin_vs_pick () : Lemma(coin () == pick [true;false]) = ()
+
